\documentclass[12pt]{article}
\usepackage{amsmath,amssymb}
\begin{document}


\paragraph{Key Point:} For a complex number $w$, the square of the modulus is 
\[
  |w|^2 \;=\; w\,\overline{w},
\]
while
\[
  w^2 \;=\; w \cdot w.
\]
These are not the same unless $w$ is purely real. In particular,
\[
  |\,2z - i\,|^2 
  \;\neq\; (2z - i)^2
  \quad\text{for complex }z.
\]

\subsection*{Detailed Explanation}

We start with the equation
\[
\bigl\lvert 2z - i \bigr\rvert 
\;=\; 
\bigl\lvert 2 + i\,z \bigr\rvert
\quad\Longleftrightarrow\quad
\bigl\lvert 2z - i \bigr\rvert^2 
\;=\; 
\bigl\lvert 2 + i\,z \bigr\rvert^2.
\]

\begin{enumerate}
\item \textbf{Incorrect Move:}  
  A common mistake is to replace
  \[
    \bigl\lvert 2z - i\bigr\rvert^2
    \quad\text{by}\quad
    (2z - i)^2.
  \]
  In fact,
  \[
    \bigl\lvert 2z - i\bigr\rvert^2
    \;=\;(2z - i)\,\overline{(2z - i)}
    \;=\;(2z - i)\bigl(2\overline{z} - \overline{i}\bigr).
  \]
  Because $\overline{i} = -\,i$, the correct expression is
  \[
    \bigl\lvert 2z - i\bigr\rvert^2 
    \;=\;
    (2z - i)\bigl(2\overline{z} + i\bigr),
  \]
  not $(2z - i)^2$.

\item \textbf{Correct Method via Real and Imag Parts:}

  Let $z = x + i\,y$, where $x,y\in\mathbb{R}$. Then:
  \[
    2z - i 
    \;=\; 2\bigl(x + i\,y\bigr) - i
    \;=\; 2x + 2i\,y - i
    \;=\; 2x \;+\; i(2y - 1).
  \]
  Hence
  \[
    \bigl\lvert 2z - i \bigr\rvert^2
    \;=\; \bigl(2x\bigr)^2 + \bigl(2y - 1\bigr)^2.
  \]
  Likewise,
  \[
    i\,z 
    \;=\; i\bigl(x + i\,y\bigr) 
    \;=\; i\,x + i^2\,y 
    \;=\; i\,x - y,
  \]
  so
  \[
    2 + i\,z 
    \;=\; 2 + (i\,x - y)
    \;=\; (2 - y) + i\,x.
  \]
  Hence
  \[
    \bigl\lvert 2 + i\,z \bigr\rvert^2
    \;=\;\bigl(2 - y\bigr)^2 + x^2.
  \]
  The original condition becomes
  \[
    4x^2 + (2y - 1)^2 
    \;=\; (2 - y)^2 + x^2.
  \]
  Expand and simplify:
  \[
    4x^2 + 4y^2 - 4y + 1 
    \;=\; x^2 + y^2 + 4 - 4y
    \;\;\Longrightarrow\;\;
    3x^2 + 3y^2 - 3 = 0
    \;\;\Longrightarrow\;\;
    x^2 + y^2 = 1.
  \]
  Therefore, the solution set in the complex plane is precisely the \emph{unit circle}:
  \[
    \bigl\{\,z : |z| = 1 \bigr\}.
  \]

\end{enumerate}

\subsection*{Conclusion}

The core error in the derivation that led to the wrong result was using $(2z - i)^2$

\end{document}